progress

src/LibEpsilon.v
@@ -39,19 +39,24 @@ Definition epsilon `{Inhab A} (P : A->Prop) : A :=
 (** ** Specification of epsilon *)
 
 Lemma epsilon_spec_exists : forall `{Inhab A} (P : A->Prop),
-  (exists x, P x) -> P (epsilon P).
+  (exists x, P x) -> 
+  P (epsilon P).
 Proof using. intros. apply~ (sig_proof (epsilon_def P)). Qed.
 
 Lemma epsilon_inv_exists : forall `{Inhab A} (P Q : A->Prop),
-  (exists x, P x) -> (forall x, P x -> Q x) -> Q (epsilon P).
+  (exists x, P x) -> 
+  (forall x, P x -> Q x) -> Q (epsilon P).
 Proof using. introv E M. apply M. apply~ epsilon_spec_exists. Qed.
 
 Lemma epsilon_spec : forall `{Inhab A} (P : A->Prop) x,
-  P x -> P (epsilon P).
+  P x -> 
+  P (epsilon P).
 Proof using. intros. apply* (epsilon_spec_exists). Qed.
 
 Lemma epsilon_inv : forall `{Inhab A} (P Q : A->Prop) x,
-  P x -> (forall x, P x -> Q x) -> Q (epsilon P).
+  P x -> 
+  (forall x, P x -> Q x) -> 
+  Q (epsilon P).
 Proof using. introv Px W. apply W. apply* epsilon_spec_exists. Qed.
 
 Lemma epsilon_eq : forall A {I:Inhab A} (P P':A->Prop),
@@ -61,16 +66,20 @@ Proof using. introv H. fequals. extens*. Qed.
 
 
 (* ---------------------------------------------------------------------- *)
-(** ** Tactics to work with [epsilon] *)
+(** ** Tactics [sets_epsilon] *)
 
-(* TODO: comment and demos *)
+(** [sets_epsilon as X]
+    [sets_epsilon in H as X]
+      
+    assigns a name [X] to an expression of the form [epsilon E]. *)
 
-Lemma epsilon_spec' : forall A (P:A->Prop) (x:A),
-  forall (H:P x) {IA:Inhab A}, P (epsilon P).
+Lemma epsilon_spec' : forall A (P:A->Prop) (x:A) (H:P x) {IA:Inhab A}, 
+  P (epsilon P).
 Proof using. intros. applys* epsilon_spec. Qed.
 
 Lemma epsilon_spec_exists' : forall A (P : A->Prop) {IA:Inhab A},
-  (exists x, P x) -> P (epsilon P).
+  (exists x, P x) -> 
+  P (epsilon P).
 Proof using. intros. applys* epsilon_spec_exists. Qed.
 
 Ltac find_epsilon cont :=
@@ -82,6 +91,33 @@ Ltac find_epsilon cont :=
 Ltac find_epsilon_in H cont :=
   match type of H with context [epsilon ?E] => cont E end.
 
+Tactic Notation "sets_epsilon" "as" ident(X) :=
+  find_epsilon ltac:(fun E => sets X: (epsilon E)).
+
+Tactic Notation "sets_epsilon" "in" hyp(H) "as" ident(X) :=
+  find_epsilon_in H ltac:(fun E => sets X: (epsilon E)).
+
+
+(* ---------------------------------------------------------------------- *)
+(** ** Tactics to work with [epsilon] *)
+
+(* LATER: produce [I] in the goal *)
+
+(** [spec_epsilon as X I]
+      => finds an expression of the form [epsilon P] in the goal,
+         names [X] this expression, and adds an hypothesis [I]
+         of type [P X]. It produces the subgoal [exists a, P a].
+
+    [spec_epsilon W as X I]
+      => same, but [W] is a witness, so the subgoal is only [P W].
+      => also works if [W] is a proof of [P a] for some [a].
+
+    [spec_epsilon as X] 
+      => same, with [I] automatically generated, of the form [HX].
+
+    [spec_epsilon in H as X I] and variants 
+      => same, but looks for [epsilon E] in hypothesis [H]. *)
+
 Ltac spec_epsilon_post E X W I :=
    first [ lets I: (>> (@epsilon_spec' _ E W) __ __)
          | lets I: (>> (@epsilon_spec' _ E _ W) __)  ];
@@ -90,17 +126,13 @@ Ltac spec_epsilon_post E X W I :=
 Ltac spec_epsilon_exists_post E X I :=
    lets I: (>> (@epsilon_spec_exists' _ E) __ __); [ | sets X: (epsilon E) ].
 
-Tactic Notation "sets_epsilon" "as" ident(X) :=
-  find_epsilon ltac:(fun E => sets X: (epsilon E)).
-
-Tactic Notation "sets_epsilon" "in" hyp(H) "as" ident(X) :=
-  find_epsilon_in H ltac:(fun E => sets X: (epsilon E)).
-
 Tactic Notation "spec_epsilon" constr(W) "as" ident(X) simple_intropattern(I) :=
   find_epsilon ltac:(fun E => spec_epsilon_post E X W I).
 
 Tactic Notation "spec_epsilon" constr(W) "in" hyp(H) "as" ident(X) simple_intropattern(I) :=
   find_epsilon_in H ltac:(fun E => spec_epsilon_post E X W I).
+
+(* LATER: missing some variants *)
 
 Tactic Notation "spec_epsilon" "as" ident(X) simple_intropattern(I) :=
   find_epsilon ltac:(fun E => spec_epsilon_exists_post E X I).
@@ -142,59 +174,67 @@ Tactic Notation "spec_epsilon" "*" "in" hyp(H) "as" ident(X) :=
 (* ********************************************************************** *)
 (** * Conversion from relations to functions *)
 
-(* Given a relation [R] of type [A->B->Prop], [choose R] returns a 
+(* Given a relation [R] of type [A->B->Prop], [rel_to_fun R] returns a 
    function [f] of type [A->B] that satisfies the relation [R], i.e.
    such that [R x (f x)] forall [x] that has an image by [R]. *)
 
-Definition choose A `{IB:Inhab B} (R:A->B->Prop) : A -> B := 
+Definition rel_to_fun A `{IB:Inhab B} (R:A->B->Prop) : A -> B := 
   fun (a:A) => epsilon (fun b => R a b).
 
-Section Choose.
+Section Rel_to_fun.
 Context (A B : Type) {IB:Inhab B}.
 Implicit Types R : A -> B -> Prop.
 
-(* TODO choose_spec and choose_unique could be reformulated using
-   incl_fr and incl_rf *)
+(* Every [a] in the domain of [R] is related by [R] with [rel_to_fun a]. *)
 
-(* Every [a] in the domain of [R] is related by [R] with [choose a]. *)
+Lemma rel_rel_to_fun_of_exists : forall R a,
+  (exists b, R a b) ->
+  R a (rel_to_fun R a).
+Proof using IB. introv [x H]. unfold rel_to_fun. applys* epsilon_spec. Qed.
 
-Lemma choose_spec : forall R a,
-  ~ (forall b, ~ R a b) ->
-  R a (choose R a).
-Proof using IB.
-  intros.
-  (* Since [a] is not a root, it has a parent [b]. *)
-  forwards [ b ? ]: exists_of_not_forall. eauto.
-  (* By definition of [choose], there follows that [choose a] is
-     well-defined, hence there is an edge from [a] to [choose a]. *)
-  unfold choose. eapply epsilon_spec. eauto.
-Qed.
-
-(* If the relation [R] is functional, then [choose a] is unique.
-   The existence of an edge from [a] to [b] implies that [b] is
-   [choose a]. *)
-
-Lemma choose_unique : forall R a b,
-  (* functional R *)
-  (forall a b1 b2, R a b1 -> R a b2 -> b1 = b2) ->
+Lemma rel_rel_to_fun_of_rel : forall R a b,
   R a b ->
-  choose R a = b.
+  R a (rel_to_fun R a).
+Proof using IB. intros. applys* rel_rel_to_fun_of_exists. Qed.
+
+Lemma rel_rel_to_fun_of_not_forall : forall R a,
+  ~ (forall b, ~ R a b) ->
+  R a (rel_to_fun R a).
 Proof using IB.
-  intros.
-  (* [R a b] implies that [a] is in the domain of [R].
-     Hence there is an edge from [a] to [choose a]. *)
-  forwards: choose_spec. rewrite not_forall_not_eq. eauto.
-  (* The result follows from the hypothesis that [R] is functional. *)
-  eauto.
+  introv. rew_logic. intros [x H]. applys* rel_rel_to_fun_of_exists.
 Qed.
 
-End Choose.
+Lemma rel_in_fun_rel_to_fun : forall R,
+  functional R ->
+  rel_in_fun R (rel_to_fun R).
+Proof using IB.
+  unfold rel_in_fun, rel_to_fun. introv M H. spec_epsilon~ y as z I. applys* M.
+Qed.
+  
+(** Reformulation of above *)
+
+Lemma rel_to_fun_eq_of_functional : forall x y R,
+  functional R ->
+  R x y -> 
+  rel_to_fun R x = y.
+Proof using IB. introv M E. applys* rel_in_fun_rel_to_fun. Qed.
+
+End Rel_to_fun.
 
 (* Remark: in the special case where [R] has type [A->A->Prop],
-   one may get away without providing a proof of [Inhab A]. *)
+   one may get away without providing a proof of [Inhab A]. 
 
-Definition choose_ A (R : A -> A -> Prop) (a : A) : A :=
-  @choose A A (Inhab_of_val a) R a.
+  Definition rel_to_fun' A (R : A -> A -> Prop) (a : A) : A :=
+    @rel_to_fun A A (Inhab_of_val a) R a.  
+*)
+
+
+
+
+
+
+
+
 
 
 
